<exercises xml:id="s_changeofbasis_ex">
  <exercisegroup>
  <introduction>
  <p>
  In each exercise a vector space <m>V</m> is given along with two ordered bases <m>B</m> and <m>B'</m>. Compute <m>\underset{B\rightarrow B'}{P}</m> and <m>\underset{B'\rightarrow B}{P}</m>.
  </p>
  </introduction>
  <exercise xml:id="ex_changebasis_twospace">
    <statement>
      <p>
      <m>V=\R^2</m>, <m>B=(\bolde_1, \bolde_2)</m>, <m>B'=\left((3,4),(1,1)\right)</m>
      </p>
    </statement>
  </exercise>
  <exercise>
    <statement>
      <p>
      <m>V=\R^2</m>, <m>B=\left((1,2), (2,1)\right)</m>, <m>B'=\left((-1,1),(1,1)\right)</m>
      </p>
    </statement>
  </exercise>
  <exercise xml:id="ex_changebasis_threespace">
    <statement>
      <p>
      <m>V=\R^3</m>, <m>B=(\bolde_1, \bolde_2, \bolde_3)</m>, <m>B'=\left( (1,0,0),(1,1,0),(1,1,1) \right)</m>
      </p>
    </statement>
  </exercise>
  <exercise xml:id="ex_changebasis_polynomials">
    <statement>
      <p>
      <m>V=P_2</m>, <m>B=(x^2, x, 1)</m>, <m>B'=((x-2)^2, (x-2), 1)</m>
      </p>
    </statement>
  </exercise>
  </exercisegroup>
<exercise>
  <statement>
    <p>
      Let <m>V=\R^3</m>, <m>B=(\bolde_1, \bolde_2, \bolde_3)</m>, <m>B'=\left( (1,0,0),(1,1,0),(1,1,1) \right)</m>, as in <xref ref="ex_changebasis_threespace"/>.
    </p>
    <ol>
      <li>
        <p>
          Compute <m>[(1,2,3)]_{B'}</m> directly using <xref ref="d_coordinatevector"/>.
        </p>
      </li>
      <li>
        <p>
          Compute <m>[(1,2,3)]_{B'}</m> using the change of basis matrix <m>\underset{B\rightarrow B'}{P}</m> and <xref ref="eq_changebasis_matrix_prop"/>.
        </p>
      </li>
    </ol>
  </statement>
</exercise>
  <exercise>
    <statement>
      <p>
        Let <m>V=P_2</m>, <m>B=(x^2, x, 1)</m>, <m>B'=((x-2)^2, (x-2), 1)</m>, as in <xref ref="ex_changebasis_polynomials"/>.
      </p>
      <ol>
        <li>
          <p>
            Compute <m>[x^2-x+4]_{B'}</m> directly using <xref ref="d_coordinatevector"/>.
          </p>
        </li>
        <li>
          <p>
            Compute <m>[x^2-x+4]_{B'}</m> using the change of basis matrix <m>\underset{B\rightarrow B'}{P}</m> and <xref ref="eq_changebasis_matrix_prop"/>.
          </p>
        </li>
      </ol>
    </statement>

</exercise>
<exercise>
  <statement>
    <p>
      Let <m>B</m> be the standard basis of <m>\R^2</m>. Find the ordered basis <m>B'</m> for which the change of basis matrix <m>\underset{B\rightarrow B'}{P}</m> is given by
      <me>\underset{B\rightarrow B'}{P}=\begin{amatrix}[rr]5\amp 1\\ -3\amp 2  \end{amatrix}
      </me>.
    </p>
  </statement>
</exercise>
<exercise>
  <statement>
      <p>
        Let <m>B</m> be the standard basis of <m>P_2</m>. Find the ordered basis <m>B'</m> for which the change of basis matrix <m>\underset{B'\rightarrow B}{P}</m> is given by
        <me>\underset{B'\rightarrow B}{P}=\begin{amatrix}[rrr]1\amp 1\amp 2\\ -3\amp 2\amp 0\\ 0\amp -1\amp 1  \end{amatrix}
        </me>.
      </p>
  </statement>
</exercise>
<exercisegroup>
<introduction>
<p>
In each exercise an inner product space <m>(V,\langle\, , \rangle)</m> is given along with two <em>orthonormal</em> ordered bases <m>B</m> and <m>B'</m>. Compute <m>\underset{B\rightarrow B'}{P}</m> and <m>\underset{B'\rightarrow B}{P}</m>. Use <xref ref="th_changebasis_orthonormal"/> to reduce your workload.
</p>
</introduction>
<exercise>
  <statement>
    <p>
      <m>V=\R^2</m> with the dot product, <m>B=\left((\sqrt{2}/2, \sqrt{2}/2), (-\sqrt{2}/2, \sqrt{2}/2)\right)</m>, <m>B'=\left( (\sqrt{3}/2, -1/2), (1/2,\sqrt{3}/2)\right)</m>
    </p>
  </statement>

</exercise>
<exercise>
  <statement>
    <p>
      <m>V=\R^4</m> with the dot product, <m>B=(\bolde_1, \bolde_2, \bolde_3, \bolde_4)</m>, <m>B'=\left(\frac{1}{2}(1,1,1,1), \frac{1}{2}(1,-1,1,-1), \frac{1}{2}(1,1,-1,-1), \frac{1}{2}(1,-1,-1,1)\right)</m>
    </p>
  </statement>

</exercise>

</exercisegroup>

  <exercise>
    <statement>
      <p>
        Suppose <m>B=(\boldv_1, \boldv_2)</m> and <m>B'=(\boldw_1, \boldw_2)</m> are two bases for the space <m>V</m> related by the change of basis matrix
        <me>
          \underset{B\rightarrow B'}{P}=\begin{amatrix}[rr]1\amp -2 \\ 3\amp 1  \end{amatrix}
        </me>.
        <ol>
          <li>
            <p>
              Let <m>\boldv=-3\boldv_1+2\boldv_2</m>. Compute <m>[\boldv]_B</m> and <m>[\boldv]_{B'}</m>.
            </p>
          </li>
          <li>
            <p>
              Let <m>\boldw=\boldw_1+2\boldw_2</m>. Compute <m>[\boldw]_B</m> and <m>[\boldw]_{B'}</m>.
            </p>
          </li>
        </ol>
      </p>
    </statement>
  </exercise>
  <exercise xml:id="ex_changebasis_three_bases">
    <statement>
      <p>
        Let <m>B</m>, <m>B'</m>, and <m>B''</m> be three ordered bases of the vector space <m>V</m>.
      </p>
      <ol>
        <li>
          <p>
            Show that
            <men xml:id="eq_changebasis_three_bases">
              \underset{B\rightarrow B''}{P}=\underset{B'\rightarrow B''}{P}\underset{B\rightarrow B'}{P}
            </men>.
            To do so, set <m>A=\underset{B'\rightarrow B''}{P}</m> and <m>B=\underset{B\rightarrow B'}{P}</m> and show that the matrix <m>AB</m> satisfies the defining property of <m>\underset{B\rightarrow B''}{P}</m>: <ie />,
            <me>
              AB[\boldv]_{B}=[\boldv]_{B''}
            </me>
            for all <m>\boldv\in V</m>.
          </p>
        </li>
        <li>
          <p>
            Using (a), show that
            <me>
              \underset{B'\rightarrow B''}{P}=\underset{B\rightarrow B''}{P}\underset{B'\rightarrow B}{P}
            </me>.
          </p>
        </li>
      </ol>
    </statement>
  </exercise>
  <exercisegroup>
  <introduction>
  <p>
  In each exercise a vector space <m>V</m> is given along with two ordered bases <m>B'</m> and <m>B''</m>.
</p>
  <ol>
    <li>
      <p>
        Compute <m>\underset{B'\rightarrow B''}{P}</m> directly using <xref ref="d_change_of_basis"/>
      </p>
    </li>
    <li>
      <p>
        Let <m>B</m> be the standard basis for <m>V</m>. Compute <m>\underset{B'\rightarrow B''}{P}</m> using formula <xref ref="eq_changebasis_three_bases"/> from <xref ref="ex_changebasis_three_bases"/>.
      </p>
    </li>
  </ol>
  </introduction>
  <exercise>
    <statement>
      <p>
        <m>V=\R^2</m>, <m>B'=\left((1,1),(1,-1)\right)</m>, <m>B''=\left((2,1),(-1,2)\right)</m>
      </p>
    </statement>
  </exercise>
  <exercise>
    <statement>
      <p>
        <m>V=P_2</m>, <m>B'=(x^2+1, x+1, 1)</m>, <m>B''=(x^2+x+1, x^2+x, x^2)</m>
      </p>
    </statement>
  </exercise>
  </exercisegroup>
  <exercise xml:id="ex_ortho_matrix_det">
    <title>Determinant of orthogonal matrices</title>
    <statement>
      <p>
        Prove: if <m>Q\in M_{nn}</m>, then <m>\det Q=\pm 1</m>.
      </p>
    </statement>
  </exercise>
  <exercise xml:id="ex_ortho_matrix_rotation_reflection">
    <statement>
      <p>
        Let <m>Q</m> be an orthogonal <m>2\times 2</m> matrix. Prove the following statements.
      </p>
      <ol>
        <li>
          <p>
            If <m>\det Q=1</m>, then <m>Q</m> is a rotation matrix: <ie />, there is a <m>\theta\in [0,2\pi]</m> such that
            <me>
              Q=\begin{amatrix}[rr] \cos\theta\amp -\sin\theta\\ \sin\theta\amp \cos\theta \end{amatrix}
            </me>.
            See <xref ref="th_transform_rotation"/>.
          </p>
        </li>
        <li>
          <p>
            If <m>\det Q=-1</m>, then <m>Q</m> is a reflection matrix: <ie />, there is a <m>\theta\in [0,\pi]</m> such that
            <me>
              Q=\begin{amatrix}[rr] \cos 2\theta\amp \sin 2\theta\\ \sin 2\theta \amp -\cos 2\theta \end{amatrix}
            </me>.
            See <xref ref="th_transform_reflection"/>.
          </p>
        </li>
      </ol>
      It is easy to verify that rotation and reflection matrices are orthogonal. We now know that conversely any orthogonal matrix is either a rotation or a reflection matrix. 
    </statement>
  </exercise>
  <exercise>
    <statement>
      <p>
        Let <m>T\colon \R^3\rightarrow \R^3</m> be the linear transformation defined as <m>T(x,y,z)=(x+2y+z, -y, x+7z)</m>. Let <m>B</m> be the standard basis of <m>\R^3</m>, and let <m>B'=\left((1,0,0), (1,1,0), (1,1,1)\right)</m>.
      </p>
      <ol>
        <li>
          <p>
            Compute <m>[T]_B</m>.
          </p>
        </li>
        <li>
          <p>
            Compute <m>[T]_{B'}</m> using <xref ref="th_change_of_basis_transformations"/>.
          </p>
        </li>
      </ol>
    </statement>
  </exercise>
  <exercise>
    <statement>
      <p>
        Let <m>T\colon P_1\rightarrow P_1</m> be the linear transformation defined as <m>T(p(x))=(x+1)p'(x)</m>. Let <m>B</m> be the standard basis of <m>P_1</m>, and let <m>B'=\left(2x+1, x-1\right)</m>.
      </p>
      <ol>
        <li>
          <p>
            Compute <m>[T]_B</m>.
          </p>
        </li>
        <li>
          <p>
            Compute <m>[T]_{B'}</m> using <xref ref="th_change_of_basis_transformations"/>.
          </p>
        </li>
      </ol>
    </statement>
  </exercise>
    <exercise>
      <title>Reflection in <m>\R^2</m></title>
      <statement>
        <p>
          Let <m>\boldv=(a,b)\in \R^2</m> be nonzero and define <m>\ell=\Span\{\boldv\}</m>, the line passing through the origin with direction vector <m>\boldv</m>. Let <m>T\colon \R^2\rightarrow \R^2</m> be reflection through <m>\ell</m>. (See <xref ref="d_reflection"/>.) In this exercise we will use a change of basis argument to find a formula for the standard matrix of <m>T</m>: <ie />, the matrix <m>A</m> satisfying <m>T(\boldx)=A\boldx</m> for all <m>\boldx\in \R^2</m>. Our answer will be expressed in terms  of <m>a</m> and <m>b</m>.
        </p>
        <ol>
          <li>
            <p>
              Pick an orthonormal basis <m>B'</m> with one vector pointing along <m>\ell</m> and compute <m>[T]_{B'}</m>.
            </p>
          </li>
          <li>
            <p>
              Let <m>B</m> be the standard basis of <m>\R^2</m>. Use <xref ref="th_change_of_basis_transformations"/> to compute <m>A=[T]_{B}</m>. (Use <xref ref="th_changebasis_orthonormal"/> to reduce your workload.)
            </p>
          </li>
          <li>
            <p>
              How do we know that <m>A</m> is the standard matrix of <m>T</m>?
            </p>
          </li>
          <li>
            <p>
              Explain why your matrix <m>A</m>, expressed in terms of <m>a</m> and <m>b</m> for <m>T</m> agrees with the matrix formula provided in <xref ref="th_transform_reflection"/>, which is expressed in terms of the angle <m>\alpha</m> that <m>\ell</m> makes with the <m>x</m>-axis.
            </p>
          </li>
        </ol>
      </statement>
    </exercise>

</exercises>
