<exercises xml:id="s_det_ex">
<exercise>
  <statement>
    <p>
      Let
      <me>
        A = \begin{bmatrix}-1\amp 1\amp 2\\ 3\amp 0\amp -5\\ 1\amp 7\amp 2 \end{bmatrix}
      </me>
      <ol>
        <li>
          <p>
            Compute <m>\det(A)</m> by expanding along the second row.
          </p>
        </li>
        <li>
          <p>
            Compute <m>\det(A)</m> by expanding along the third column.
          </p>
        </li>
      </ol>
    </p>
  </statement>
</exercise>
<exercisegroup>
<introduction>
  <p>
    Compute the determinant of the given matrix. Indicate which row or column you expand along.
  </p>
</introduction>
<exercise>
  <statement>
    <p>
      <me>
        A=\begin{amatrix}[rrr]2\amp 0\amp 3\\ 0\amp 3\amp 2\\ -2\amp 0\amp -4 \end{amatrix}
      </me>

    </p>
  </statement>
</exercise>
<exercise>
  <statement>
    <p>
      <me>
        A=\begin{amatrix}[rrrr] 2\amp 1\amp 0\amp 5\\ 1\amp 2\amp 0\amp -1\\ 1\amp 4\amp -3\amp 0\\ 2\amp 6\amp 3\amp 2 \end{amatrix}
      </me>

    </p>
  </statement>
</exercise>
<exercise>
  <statement>
    <p>
      <me>
        A=\begin{amatrix}[rrrrr]4\amp 0\amp 0\amp 1\amp 0\\ 3\amp 3\amp 3\amp -1\amp 0\\ 1\amp 2\amp 4\amp 2\amp 3\\ 9\amp 4\amp 6\amp 2\amp 3\\ 2\amp 2\amp 4\amp 2\amp 3 \end{amatrix}
      </me>

    </p>
  </statement>
</exercise>
</exercisegroup>
<exercise>
  <statement>
    <p>
      Let
      <me>
        A=\begin{amatrix}[rrrr]1\amp -3\amp 1\amp 1\\ -3\amp 1\amp 1\amp 1\\ 1\amp 1\amp -3\amp 1\\ 1\amp 1\amp 1\amp -3 \end{amatrix}
      </me>.
      Show <m>\det A=0</m> without computing its determinant directly by expansion along a row or column. In other words, use a row reduction technique or <xref ref="th_invertibility_expanded"/>.
    </p>
  </statement>
  <solution>
    <p>

    </p>
  </solution>
</exercise>
<exercise>
  <statement>
    <p>
      Let <m>A</m> be an <m>n\times n</m> matrix, and let <m>c</m> be a scalar.
      State and prove a formula relating <m>\det(cA)</m> with <m>\det(A)</m>.
    </p>
  </statement>
  <solution>
    <p>
      Warning: in general <m>\det(cA)\ne c\det(A)</m>!
      We claim in fact that if <m>A</m> is <m>n\times n</m>, then <m>\det(cA)=c^n\det(A)</m>. We give two proofs: one uses only induction and the definition of the determinant; the other uses the multiplicative property of the determinant.
    </p>
    <proof>
      <title>Proof by induction</title>
      <p>
        We show that for all <m>n\geq 1</m>, if <m>A</m> is an <m>n\times n</m> matrix, then <m>\det(cA)=c^n\det A</m>.
      </p>
      <case>
       <title>Base step: <m>n=1</m></title>
      <p>
      Here we have <m>A=[a]</m>, <m>cA=[ca]</m>, and thus <m>\det(cA)=ca=c\det A</m>.
      </p>
      </case>
      <case>
       <title>Induction step</title>
      <p>
      We assume that <m>\det(cB)=c^n\det B</m> for any <m>n\times n</m> matrix <m>B</m>, and prove <m>\det(cA)=c^{n+1}\det A</m> for any <m>(n+1)\times (n+1)</m> matrix <m>A</m>. To this end, let <m>A=[a_{ij}]_{(n+1)\times (n+1)}</m>. Then
      <md>
        <mrow>\det(cA) \amp =\det [ca_{ij}]_{(n+1)\times (n+1)} </mrow>
        <mrow> \amp = \sum_{j=1}^{n+1}(-1)^{1+j}ca_{1j}\det(c\widetilde{A}_{1j})</mrow>
        <mrow>  \amp = \sum_{j=1}^{n+1}(-1)^{1+j}ca_{1j}(c^n \det\widetilde{A}_{1j}) \amp (\text{induction})</mrow>
        <mrow>  \amp = c^{n+1}\sum_{j=1}^{n+1}(-1)^{1+j}a_{1j}\det\widetilde{A}_{1j}</mrow>
        <mrow>  \amp =c^{n+1}\det A</mrow>
      </md>.
      </p>
      </case>
    </proof>
    <proof>
      <title>Proof using determinant properties</title>
      <p>
        We have <me>
          cA=(cI)A=\begin{bmatrix}c\amp 0\amp \dots\amp 0\\ 0\amp c\amp 0\amp \dots\\ \vdots \amp \\ 0\amp 0\amp \dots\amp c \end{bmatrix} A
        </me>.
        Then
        <md>
          <mrow>\det(cA) \amp=\det((cI)A) </mrow>
          <mrow> \amp =\det(cI)\, \det A\amp (<xref ref="th_det_mult"/>) </mrow>
          <mrow>  \amp =(\underset{n \text{times}}{\underbrace{c\cdot c\cdots c}})\,\det A \amp (<xref ref="th_det_triangular"/>) </mrow>
          <mrow>  \amp =c^n\det A </mrow>
        </md>.
      </p>
    </proof>

  </solution>
</exercise>
<exercise>
  <statement>
    <p>
      Let <m>A</m> and <m>B</m> be <m>n\times n</m> matrices,
      and suppose <m>B</m> is invertible.
      Prove the following:
    </p>
    <ol>
      <li>
        <p>
          <m>\ds \det(B^{-1})=\frac{1}{\det(B)}</m>.
        </p>
      </li>
      <li>
        <p>
          <m>\ds \det(B^{-1}AB)=\det(A)</m>.
        </p>
      </li>
    </ol>
  </statement>
</exercise>
<exercise>
  <statement>
    <p>
      In our proof of statement (2) of <xref ref="th_det_zero_repeated_row"/> we only showed that if <m>A</m> is a square matrix with two identical rows, then <m>\det A=0</m>. Assuming this, show that the same is true if <m>A</m> has two identical columns.
    </p>
  </statement>
</exercise>
<exercise>
  <statement>
    <p>
      State and prove an analogue to <xref ref="th_det_row_ops"/> that describes how the corresponding <em>column operations</em> (i.e., scale a column by <m>c</m>, swap two columns, column addition) affect the determinant of a matrix.
    </p>
  </statement>
  <hint>
    <p>
      Express each of these types of column operations as multiplication on the right by an elementary matrix.
    </p>
  </hint>
</exercise>
<exercise>
  <statement>
    <p>
      Let <m>A</m> be the <m>n\times n</m> matrix with <m>a's</m> along the diagonal and <m>b</m>'s elsewhere: i.e.,
      <me>
        A=\begin{bmatrix}a\amp b\amp b\dots \\ b\amp a\amp b\amp \dots\\ \vdots \amp  \amp \vdots \\ b\amp b\amp \dots \amp a \end{bmatrix}
      </me>.
      State and prove a formula for <m>\det A</m>.
      Look at the <m>n=2</m> and <m>n=3</m> cases first.
      To prove the formula in the general case you may want to make use of row reduction and <xref ref="th_det_row_ops"/>.
    </p>
  </statement>
</exercise>
<exercise>
  <statement>
    <p>
      Given scalars <m>r_1, r_2, \dots, r_n\in \R</m> the <em>Vandermonde</em> matrix is defined as
      <me>
        A_{r_1,r_2,\dots, r_n}=\begin{bmatrix}1\amp 1\amp \cdots \amp 1\\ r_1\amp r_2\amp \cdots \amp  r_n\\ r_1^2\amp r_2^2\amp \cdots \amp r_n^2\\ \vdots \amp  \vdots \amp \cdots \amp \vdots\\ r_1^{n-1}\amp r_2^{n-1}\amp \cdots \amp r_n^{n-1} \end{bmatrix}
      </me>.
      In other words, we have
      <me>
        (A_{r_1,r_2,\dots, r_n})_{ij}=r_j^{i-1}
      </me>
      Prove:
      <me>\ds\det (A_{r_1,r_2,\dots,
      r_n})=\prod_{1\leq i\lt j\leq n}(r_j-r_i)</me>.
    </p>
  </statement>
</exercise>
</exercises>
