<section xmlns:xi="http://www.w3.org/2001/XInclude" xml:id="s_orthogonal_projection">
  <title>Orthogonal complements and orthogonal projection</title>
  <subsection>
  <title>Orthogonal complement</title>
  <definition xml:id="d_orthogonal_complement">
    <title>Orthogonal complement</title>
    <idx><h>orthogonal</h><h>complement (of a subspace)</h></idx>
    <notation>
      <usage><m>W^\perp</m></usage>
      <description>the orthogonal complement of <m>W</m></description>
    </notation>
    <statement>
      <p>.
        Let <m>(V,\langle \ , \rangle)</m> be an inner product vector space,
        and let <m>W\subseteq V</m> be a subspace.
        The <term>orthogonal complement of <m>W</m></term>, denoted <m>W^\perp</m>, is defined as
        <me>
          W^\perp=\{\boldv\in V\colon \langle \boldv, \boldw\rangle=0 \text{ for all } \boldw\in W\}
        </me>.
        In other words <m>W^\perp</m> is the set of vectors that are orthogonal to
        <term>all</term> elements of <m>W</m>.
      </p>
    </statement>
  </definition>
  <theorem xml:id="th_orthogonal_complement">
    <title>Orthogonal complement</title>
    <statement>
      <p>
        Let <m>(V,\langle \ , \rangle)</m> be an inner product vector space,
        and let <m>W\subseteq V</m> be a subspace.
        <ol>
          <li>
            <p>
              The orthogonal complement <m>W^\perp</m> is a subspace of <m>V</m>.
            </p>
          </li>
          <li>
            <p>
              We have <m>W\cap W^\perp=\{\boldzero\}</m>.
            </p>
          </li>
          <li>
            <p>
              If <m>\dim V=n\lt \infty</m> then
              <me>
                \dim W+\dim W^\perp=n
              </me>.
            </p>
          </li>
        </ol>
      </p>
    </statement>
  </theorem>
  <example>
    <statement>
      <p>
        Consider the inner product space <m>\R^3</m> with the dot product. Let <m>W=\Span\{(1,1,1)\}\subset \R^3</m>, the line
        passing through the origin with direction vector <m>(1,1,1)</m>.
        The orthogonal complement <m>W^\perp</m> is the set of vectors orthogonal to <m>(1,1,1)</m>. Using the definition of dot product, this is the set of solutions <m>(x,y,z)</m> to the equation
        <me>
          x+y+z=0
        </me>,
          which we recognize as the plane passing through the origin with normal vector <m>(1,1,1)</m>. Note that we have
          <me>
            \dim W+\dim W^\perp=1+2=3,
          </me>
          as predicted in <xref ref="th_orthogonal_complement"/>.

      </p>
    </statement>
  </example>
    <p>
      The notion of orthogonal complement gives us a more conceptual way of understanding the relationship between the various fundamental spaces of a matrix.
    </p>
    <theorem>
      <statement>
        <p>
          Let <m>A</m> be <m>m\times n</m>,
          and consider <m>\R^n</m> and <m>\R^m</m> as inner product spaces with respect to the dot product.
          Then:
          <ol>
            <li>
              <p>
                <m>\NS(A)=\left(\RS(A)\right)^\perp</m>,
                and thus <m>\RS(A)=\left(\NS(A)\right)^\perp</m>.
              </p>
            </li>
            <li>
              <p>
                <m>\NS(A^T)=\left(\CS(A)\right)^\perp</m>,
                and thus <m>\CS(A)=\left(\NS(A^T)\right)^\perp</m>.
              </p>
            </li>
          </ol>
        </p>
      </statement>
      <proof>
        <ol>
          <li>
            <p>
              Using the dot product method of matrix multiplication,
              we see that a vector <m>\boldv\in\NS(A)</m> if and only if
              <m>\boldv\cdot\boldr_i=0</m> for each row <m>\boldr_i</m> of <m>A</m>.
              Since the <m>\boldr_i</m> span <m>\RS(A)</m>,
              the linear properties of the dot product imply that <m>\boldv\cdot\boldr_i=0</m> for each row
              <m>\boldr_i</m> of <m>A</m> if and only if <m>\boldv\cdot\boldw=0</m> for <em>all</em>
              <m>\boldw\in\RS(A)</m> if and only if <m>\boldv\in \RS(A)^\perp</m>.
            </p>
          </li>
          <li>
            <p>
              This follows from (1) and the fact that <m>\CS(A)=\RS(A^T)</m>.
            </p>
          </li>
        </ol>
      </proof>
    </theorem>

    <example>
      <statement>
        <p>
          Understanding the orthogonal relationship between <m>\NS(A)</m> and <m>\RS(A)</m> allows us in many cases to quickly determine/visualize the one from the other. As an example, consider <m>A=\begin{bmatrix}1\amp -1\amp 1\\ 1\amp -1\amp -1 \end{bmatrix}</m>. Looking at the columns, we see easily that <m>\rank(A)=2</m>,
          which implies that <m>\nullity(A)=3-2=1</m>.
          Since <m>(1,-1,0)</m> is an element of <m>\NS(A)</m> and <m>\dim(\NS(A))=1</m>,
          we must have <m>\NS(A)=\Span\{(1,-1,0)\}</m>, a line. By orthogonality, we conclude that
          <me>
            \RS(A)=\NS(A)^\perp=\text{ (plane perpendicular to \((1,-1,0)\)) }
          </me>.
        </p>
      </statement>
    </example>
  </subsection>
  <subsection>
    <title>Orthogonal Projection</title>
    <theorem xml:id="th_orthogonal_projection">
      <title>Orthogonal projection theorem</title>
      <statement>
        <p>
          Let <m>(V,\langle \ , \rangle)</m> be an inner product space,
          and let <m>W\subseteq V</m> be a
          <em>finite-dimensional</em> subspace.
          <ol>
            <li>
              <title>Orthogonal decomposition</title>
              <p>
                For all <m>\boldv\in V</m> there is a unique choice of vectors <m>\boldw\in W</m> and
                <m>\boldw^\perp\in W^\perp</m> such that <m>\boldv=\boldw+\boldw^\perp</m>.
                We call this vector expression an
                <term>orthogonal decomposition</term> of <m>\boldv</m>,
                and denote <m>\boldw=\proj{\boldv}{W}</m> and <m>\boldw^\perp=\proj{\boldv}{W^\perp}</m>,
                the <term>orthogonal projections</term>
                of <m>\boldv</m> onto <m>W</m> and <m>W^\perp</m>, respectively.
              </p>
            </li>
            <li>
              <title>Distance to <m>W</m></title>
              <p>
                The orthogonal projection <m>\boldw=\proj{\boldv}{W}</m> is the unique element of <m>W</m> that <em>minimizes</em> the distance to <m>\boldv</m>.
                In other words
                <me>\norm{\boldv-\proj{\boldv}{W}}\leq\norm{\boldv-\boldw'}
                </me>
                for all <m>\boldw'\in W</m>.
              </p>
              <p>
                Accordingly, we define the <term>distance from <m>\boldv</m> to <m>W</m></term>, denoted <m>d(\boldw, W)</m>, as
                <me>
                d(\boldv, W)=d(\boldv, \proj{\boldv}{W}=\norm{\boldw^\perp}
                </me>.
              </p>
            </li>
            <li>
              <title>Orthogonal projection formula</title>
              <p>
                Pick an <em>orthogonal</em> basis <m>B=\{\boldv_1,\boldv_2,\dots, \boldv_r\}</m> of <m>W</m>.
                Then
                <me> \proj{\boldv}{W}=\sum_{i=1}^r\frac{\angvec{\boldv,\boldv_i}}{\angvec{\boldv_i, \boldv_i}}\boldv_i
                </me>.
              </p>
            </li>
          </ol>
        </p>
      </statement>
    </theorem>
  </subsection>
  <subsection>
  <title>Proof of orthogonal projection theorem</title>
  <p>
    Pick an <em>orthogonal</em> basis
    <m>B=\{\boldv_1,\boldv_2,\dots, \boldv_r\}</m> of <m>W</m> and set <m>\boldw=\sum_{i=1}^r\frac{\angvec{\boldv,\boldv_i}}{\angvec{\boldv_i, \boldv_i}}\boldv_i</m>.
    This is clearly an element of <m>W</m>.
    Next we set <m>\boldw^\perp=\boldv-\boldw=\boldv-\sum_{i=1}^r\frac{\angvec{\boldv,\boldv_i}}{\angvec{\boldv_i, \boldv_i}}\boldv_i</m>.
  </p>
  <p>
    To complete the proof, we must show the following: (A)
    <m>\boldw^\perp\in W^\perp</m>, (B) this choice of <m>\boldw</m> and <m>\boldw^\perp</m> is unique,
    and (C) <m>\boldw</m> is the closest element of <m>W</m> to <m>\boldv</m>.
  </p>
  <subsection>
    <title>(A)</title>
    <p>
      For all <m>i</m> we have
    </p>
  </subsection>
  <md>
    <mrow>\langle\boldw^\perp,\boldv_i\rangle\amp =\amp \langle \boldv-\sum_{i=1}^r\frac{\angvec{\boldv,\boldv_i}}{\angvec{\boldv_i, \boldv_i}}\boldv_i, \boldv_i\rangle</mrow>
    <mrow>\amp =\amp \langle \boldv, \boldv_i\rangle-\langle \sum_{i=1}^r\frac{\angvec{\boldv,\boldv_i}}{\angvec{\boldv_i, \boldv_i}}\boldv_i ,\boldv_i\rangle \hspace{9pt} \text{ (distr.) }</mrow>
    <mrow>\amp =\amp \langle \boldv, \boldv_i\rangle-\frac{\angvec{\boldv,\boldv_i}}{\angvec{\boldv_i,\boldv_i}}\langle\boldv_i,\boldv_i\rangle \hspace{9pt} \text{ (by orthogonality) }</mrow>
    <mrow>\amp =\amp 0</mrow>
  </md>
  <subsection>
    <title>(B)+(C)</title>
    <p>
      Recall: <m>\boldw</m> satisfies <m>\boldv=\boldw+\boldw^\perp</m>,
      where <m>\boldw^\perp\in W^\perp</m>.
      Now take any other <m>\boldw'\in W</m>.
      Then
    </p>
  </subsection>
  <md>
    <mrow>\norm{\boldv-\boldw'}^2\amp =\amp \norm{\boldw^\perp+(\boldw-\boldw')}^2
    =\norm{\boldw^\perp}^2+\norm{\boldw-\boldw'}^2 \hspace{9pt} \text{ (Pythag. theorem) }</mrow>
    <mrow>\amp \geq\amp  \norm{\boldw^\perp}^2=\norm{\boldv-\boldw}^2</mrow>
  </md>.
  <p>
    Taking square-roots now proves the desired inequality.
    Furthermore, we have <em>equality</em>
    iff the last inequality is an equality iff
    <m>\norm{\boldw''}=\norm{\boldw-\boldw'}=0</m> iff <m>\boldw=\boldw'</m>.
    This proves our choice of <m>\boldw</m> is the <em>unique</em>
    element of <m>W</m> minimizing the distance to <m>\boldv</m>!
  </p>
  </subsection>
  <corollary xml:id="cor_orthocomp_selfdual">
    <statement>
      <p>
        Let <m>(V,\angvec{\ , \ })</m> be an inner product space,
        and let <m>W\subseteq V</m> be a finite-dimensional subspace.
        Then <m>(W^\perp)^\perp=W</m>.
      </p>
    </statement>
  </corollary>
  <proof>
    <p>
      Clearly <m>W\subseteq (W^\perp)^\perp</m>.
      For the other direction, take <m>\boldv\in (W^\perp)^\perp</m>.
      Using the <em>orthogonal projection theorem</em>,
      we can write <m>\boldv=\boldw+\boldw^\perp</m> with
      <m>\boldw\in W</m> and <m>\boldw^\perp\in W^\perp</m>.
      We will show <m>\boldw^\perp=\boldzero</m>.
    </p>
    <p>
      Since <m>\boldv\in (W^\perp)^\perp</m> we have <m>\angvec{\boldv,\boldw^\perp}=0</m>.
      Then we have
      <md>
        <mrow>0\amp =\angvec{\boldv,\boldw^\perp}</mrow>
        <mrow>\amp =\angvec{\boldw+\boldw^\perp,\boldw^\perp}</mrow>
        <mrow>\amp =\angvec{\boldw,\boldw^\perp}+\angvec{\boldw^\perp,\boldw^\perp} \amp \text{ (since \(W\perp W^\perp\)) }</mrow>
        <mrow>\amp =0+\angvec{\boldw^\perp,\boldw^\perp}</mrow>
      </md>
    </p>
    <p>
      Thus <m>\angvec{\boldw^\perp,\boldw^\perp}=0</m>.
      It follows that <m>\boldw^\perp=\boldzero</m>,
      and hence <m>\boldv=\boldw+\boldzero=\boldw\in W</m>.
    </p>
  </proof>
  <corollary xml:id="cor_orthoproj_linear">
    <statement>
      <p>
        Let <m>(V,\angvec{\ , \ })</m> be an inner product space,
        and let <m>W\subseteq V</m> be a finite-dimensional subspace.
      </p>
      <p>
        Define <m>T\colon V\rightarrow V</m> as <m>T(\boldv)=\proj{\boldv}{W}</m>.
        Then <m>T</m> is a linear transformation.
      </p>
      <p>
        In other words,
        orthogonal projection onto <m>W</m> defines a linear transformation of <m>V</m>.
      </p>
    </statement>
  </corollary>
  <proof>
    <p>
      We must show that <m>T(c\boldv_1+d\boldv_2)=cT(\boldv_1)+dT(\boldv_2)</m> for all
      <m>c,d\in\R</m> and <m>\boldv_1,\boldv_2\in V</m>.
      This is easily shown by picking an orthonormal basis
      <m>B=\{\boldv_1,\boldv_2, \dots, \boldv_r\}</m> of <m>W</m> and using the formula from the orthogonal projection theorem.
    </p>
  </proof>
  <subsection>
    <title>Projection onto lines and planes in $\R^3$</title>
    <p>
      Let's revisit orthogonal projection onto lines and planes in <m>\R^3</m> passing through the origin.
      Here the relevant inner product is dot product.
    </p>
  </subsection>
  <subsection>
    <title>Projection onto a line $\ell$</title>
    <p>
      Any line in <m>\R^3</m> passing through the origin can be described as <m>\ell=\Span\{\boldv_0\}</m>,
      for some <m>\boldv_0=(a,b,c)\ne 0</m>.
      Since this is an orthogonal basis of <m>\ell</m>,
      by the orthogonal projection theorem we have,
      for any <m>\boldv=(x,y,z)</m>
      <me>
        \proj{\boldv}{\ell}=\frac{\boldv\cdot \boldv_0}{\boldv_0\cdot\boldv_0}\boldv_0=\frac{ax+by+cz}{a^2+b^2+c^2}(a,b,c)=\frac{1}{a^2+b^2+c^2}\begin{bmatrix}a^2\amp ab\amp ac\\ ab\amp b^2\amp bc\\ ac\amp bc\amp c^2 \end{bmatrix} \begin{bmatrix}x\\ y\\ z \end{bmatrix}
      </me>.
    </p>
    <p>
      We have re-derived the matrix formula for orthogonal projection onto <m>\ell</m>.
    </p>
  </subsection>
  <subsection>
    <title>Projection onto lines and planes in $\R^3$</title>
    <p>
      Let's revisit orthogonal projection onto lines and planes in <m>\R^3</m> passing through the origin.
      Here the relevant inner product is dot product.
    </p>
  </subsection>
  <subsection>
    <title>Projection onto a plane</title>
    <p>
      Any plane in <m>\R^3</m> passing through the origin can be described with the equation
      <m>\mathcal{P}\colon ax+by+cz=0</m> for some <m>\boldn=(a,b,c)\ne 0</m>.
      This says precisely that <m>\mathcal{P}</m> is the orthogonal complement of the line <m>\ell=\Span\{(a,b,c)\}</m>:
      i.e., <m>\mathcal{P}=\ell^\perp</m>.
    </p>
    <p>
      From the orthogonal projection theorem, we know that
      <me>
        \boldv=\proj{\boldv}{\ell}+\proj{\boldv}{\ell^\perp}=\proj{\boldv}{\ell}+\proj{\boldv}{\mathcal{P}}
      </me>.
    </p>
    <p>
      But then
      <me>
        \proj{\boldv}{\mathcal{P}}=\boldv-\proj{\boldv}{\ell}=I \ \boldv-\proj{\boldv}{\ell}=(I-A)\boldv
      </me>,
      where <m>A</m> is the matrix formula for
      <m>\proj{\boldv}{\ell}</m> from the previous example.
      We conclude that the matrix defining <m>\proj{\boldv}{\mathcal{P}}</m> is
      <me>
        I-\frac{1}{a^2+b^2+c^2}\begin{bmatrix}a^2\amp ab\amp ac\\ ab\amp b^2\amp bc\\ ac\amp bc\amp c^2 \end{bmatrix} = \frac{1}{a^2+b^2+c^2}\begin{bmatrix}b^2+c^2\amp -ab\amp -ac\\ -ab\amp a^2+c^2\amp -bc\\ -ac\amp -bc\amp a^2+b^2 \end{bmatrix}
      </me>
    </p>
  </subsection>
  <p>
    We can express this in terms of matrix multiplication as
  </p>
  <p>
    \item Translate the whole picture by <m>-Q=(-q_1,-q_2, -q_3)</m>,
    which means we replace <m>P=(x,y,z)</m> with
    <m>P-Q=(x-q_1,y-q_2,z-q_3)</m>. \item Apply our formulas from before,
    replacing <m>(x,y,z)</m> with
    <m>(x-q_1,y-q_2,z-q_3)</m> \item Translate back by adding <m>Q</m> to your answer.
  </p>
  <subsection>
    <title>Example: sine/cosine series</title>
    <p>
      Let <m>V=C[0,2\pi]</m> with inner product <m>\langle f, g\rangle=\int_0^{2\pi}f(x)g(x) \, dx</m>.
    </p>
    <p>
      We have seen that the set
      <me>
        B=\{1, \cos(x),\sin(x),\cos(2x),\sin(2x), \dots , \cos(nx),\sin(nx)\}
      </me>
      is orthogonal.
      Thus <m>B</m> is an orthogonal basis of <m>W=\Span(B)</m>,
      which we might describe as the space of
      <term>trigonometric polynomials of degree at most <m>n</m></term>.
    </p>
    <p>
      Given an arbitrary function <m>f(x)\in C[0,2\pi]</m>,
      its orthogonal projection onto <m>W</m> is the function
      <me>
        \hat{f}(x)=a_0+a_1\cos(x)+b_1\sin(x)+a_2\cos(2x)+b_2\sin(2x)+\cdots +a_n\cos(nx)+b_n\sin(nx)
      </me>,
      where
      <me>
        a_0=\frac{1}{2\pi}\int_0^{2\pi} f(x) \ dx, \ a_j=\frac{1}{\pi}\int_0^{2\pi}f(x)\cos(jx)\, dx, \ b_k=\frac{1}{\pi}\int_0^{2\pi}f(x)\sin(kx)\, dx
      </me>.
    </p>
    <p>
      The projection theorem tells us that <m>\hat{f}</m> is the
      <q>best</q>
      trigonometric polynomial approximation of <m>f(x)</m>
      (of degree at most <m>n</m>),
      in the sense that for any other sinusoidal <m>g\in W</m>,
      <m>\left\vert\left\vert f-\hat{f}\right\vert\right\vert\leq \norm{f-g}</m>.
    </p>
    <p>
      This means in turn
      <me>
        \int_0^{2\pi} (f-\hat{f})^2\, dx\leq \int_0^{2\pi} (f-g)^2 \, dx
      </me>.
    </p>
  </subsection>
  <subsection>
    <title>Example: least-squares solution to $A\boldx=\boldy$</title>
    <p>
      Often in applications we have an
      <m>m\times n</m> matrix <m>A</m> and vector
      <m>\boldy\in\R^m</m> for which the matrix equation
      <me>
        A\boldx=\boldy
      </me>
      has no solution.
      In terms of fundamental spaces,
      this means simply that <m>\boldy\notin \CS(A)</m>.
      Set <m>W=\CS(A)</m>.
    </p>
    <p>
      In such situations we speak of a <em>least-squares</em>
      solution to the matrix equation.
      This is a vector <m>\hat{\boldx}</m> such that <m>A\hat{\boldx}=\hat{\boldy}</m>,
      where <m>\hat{\boldy}=\proj{\boldy}{W}</m>.
      Here the inner product is taken to be the dot product.
    </p>
    <p>
      Note: the equation <m>A\hat{\boldx}=\hat{\boldy}</m> is guaranteed to have a solution since
      <m>\hat{\boldy}=\proj{\boldy}{W}</m> lies in <m>\CS(A)</m>.
    </p>
    <p>
      The vector <m>\hat{\boldx}</m> is called a least-square solutions because its image
      <m>\hat{\boldy}</m> is the element of <m>\CS(A)</m> that is
      <q>closest</q>
      to <m>\boldy</m> in terms of the dot product.
      Writing <m>\boldy=(y_1,y_2,\dots,y_n)</m> and <m>\hat{\boldy}=(y_1',y_2',\dots,
      y_n')</m>,
      this means that <m>\hat{\boldy}</m> minimizes the distance
      <me>
        \norm{\boldy-\hat{\boldy}}=\sqrt{(y_1-y_1')^2+(y_2-y_2')^2+\cdots +(y_n-y_n')^2}
      </me>.
    </p>
  </subsection>
  <subsection>
    <title>Least-squares example (curve fitting)</title>
    <p>
      Suppose we wish to find an equation of a line <m>y=mx+b</m> that best fits
      (in the least-square's sense)
      the following <m>(x,y)</m> data points:
      <m>P_1=(-3,1), P_2=(1,2), P_3=(2,3)</m>.
    </p>
    <p>
      Then we seek <m>m</m> and <m>b</m> such that
      <md>
        <mrow>1\amp =m(-3)+b</mrow>
        <mrow>2\amp =m(1)+b</mrow>
        <mrow>3\amp =m(2)+b</mrow>
      </md>,
      or equivalently,
      we wish to solve <m>\begin{bmatrix}-3\amp 1\\ 1\amp 1\\ 2\amp 1 \end{bmatrix} \begin{bmatrix}m \\ b \end{bmatrix} =\begin{bmatrix}1\\ 2\\ 3 \end{bmatrix}</m>.
    </p>
    <p>
      This equation has no solution as
      <m>\boldy=(1,2,3)</m> does no lie in <m>W=\CS(A)=\Span(\{(-3,1,2),(1,1,1)\}</m>.
      So instead we compute <m>\hat{\boldy}=\proj{\boldy}{W}=(13/14,33/14,38/14)</m>. (This was not hard to compute as conveniently the given basis of <m>W</m> was already orthogonal!)
    </p>
    <p>
      Finally we solve <m>A\begin{bmatrix}m\\ b \end{bmatrix} =\hat{\boldy}</m>,
      getting <m>m=5/14</m>, <m>b=28/14=2</m>.
      Thus <m>y=\frac{5}{14}x+2</m> is the line best fitting the data in the least-squares sense.
    </p>
  </subsection>
  <subsection>
    <title>Least-squares example contd.</title>
    <p>
      In what sense does <m>y=\frac{5}{14}x+2</m>
      <q>best</q>
      fit the data?
      <!-- <me>
        <image width="37%" source="images/LeastSquares.png"/>
      </me> -->
    </p>
    <p>
      Let <m>\boldy=(1,2,3)=(y_1,y_2,y_3)</m> be the given <m>y</m>-values of the points,
      and <m>\hat{\boldy}=(y_1',y_2',y_3')</m> be the projection we computed before.
      In the graph the values <m>\epsilon_i</m> denote the vertical difference
      <m>\epsilon_i=y_i-y_i'</m> between the data points, and our fitting line.
    </p>
    <p>
      The projection <m>\hat{\boldy}</m> makes the error
      <m>\norm{\boldy-\hat{\boldy}}=\sqrt{ \epsilon_1^2+\epsilon_2^2+\epsilon_3^2}</m> as small as possible.
    </p>
    <p>
      This means if I draw <em>any other line</em>
      and compute the corresponding differences
      <m>\epsilon_i'</m> at the <m>x</m>-values -3, 1 and 2, then we have
      <me>
        \epsilon_1^2+\epsilon_2^2+\epsilon_3^2\leq (\epsilon_1')^2+(\epsilon_2')^2+(\epsilon_3')^2
      </me>
    </p>
  </subsection>
  <subsection>
  <title>Finding least squares solutions</title>
  <p>
    As the last example illustrated,
    one method of finding a least-squares solution <m>\boldx</m> to
    <m>A\boldx=\boldy</m> is to first produce an orthogonal basis for <m>\CS(A)</m>,
    then compute <m>\hat{\boldy}=\proj{\boldy}{\CS(A)}</m>,
    and then use GE to solve <m>A\boldx=\hat{\boldy}</m>.
  </p>
  <p>
    Alternatively, it turns out
    (through a little trickery)
    that <m>\hat{\boldy}=A\boldx</m>,
    where <m>\boldx</m> is a solution to the equation
    <me>
      A^TA\boldx=A^T\boldy
    </me>.
  </p>
  <p>
    This solves us the hassle of computing an orthogonal basis for <m>\CS(A)</m>;
    to find a least-squares solution <m>\boldx</m> for <m>A\boldx=\boldy</m>,
    we simply use GE to solve the boxed equation. (Some more trickery shows a solution is guaranteed to exist!)
  </p>
  <subsection>
    <title>Example</title>
    <p>
      In the previous example we were seeking a least-squares solution
      <m>\boldx=\colvec{m\\ b}</m> to <m>A\boldx=\boldy</m>,
      where <m>A=\begin{bmatrix}-3\amp 1\\ 1\amp 1\\ 2\amp 1 \end{bmatrix} , \boldy=\colvec{1\\2\\3}</m>.
    </p>
  </subsection>
  <p>
    The equation <m>A^TA\boldx=A^T\boldy</m> is thus
    <me>
      \begin{bmatrix}14\amp 0\\ 0\amp 3 \end{bmatrix} \boldx= \colvec{5\\ 6}
    </me>
  </p>
  <p>
    As you can see,
    <m>\boldx=\colvec{m\\ b}=\colvec{5/14\\ 2}</m> is a least-squares solution,
    just as before
  </p>
  </subsection>
  <!-- <xi:include href="./s_orthogonal_projection_ex.ptx"/> -->
</section>
