<section xmlns:xi="http://www.w3.org/2001/XInclude" xml:id="s_proof_technique">
<title>Proof techniques</title>
<introduction>
  Proof writing is an art, a technical skill you will hone and refine throughout your career; and like any art, proof writing has many tricks of the trade. We gather a few here in the form of a collection of general proof techniques. Part of mastering these techniques involves understanding the circumstances where they can be of use. When selecting a technique, we are guided in part by the logical structure and particular mathematical content of the proposition under consideration. The proof techniques below are organized under this guiding principle.
</introduction>
<subsection xml:id="ss_logical_structure">
  <title>Logical structure</title>
  <subsubsection xml:id="sss_implication">
    <title>Implication</title>
    <p>
      By <xref ref="d_logical_ops"/> the only time an implication  <m>\mathcal{P}\implies\mathcal{Q}</m> is false is when <m>\mathcal{P}</m> is true and <m>\mathcal{Q}</m> is false. Accordingly, the <em>direct approach</em> to proving an implication <m>\mathcal{P}\implies \mathcal{Q}</m> is to assume <m>\mathcal{P}</m> is true, and use this assumption to prove <m>\mathcal{Q}</m> is true.
  </p>
  <p>
    A common <em>indirect approach</em> used to prove an implication <m>\mathcal{P}\implies \mathcal{Q}</m> is to prove its <em>contrapositive</em>  <m>\neg\mathcal{Q}\implies \neg \mathcal{P} </m>, which is logically equivalent to the original implication. In this case we assume <m>\mathcal{Q}</m> is not true, and show <m>\mathcal{P}</m> is not true. (Exercise: use a truth table to show the contrapositive is logically equivalent to the original implication.)
  </p>
  <warning>
    <statement>
      <p>
        The <em>converse</em> of an implication <m>\mathcal{P}\implies \mathcal{Q}</m> is the implication <m>\mathcal{Q}\implies \mathcal{P}</m>; the <em>inverse</em> of <m>\mathcal{P}\implies\mathcal{Q}</m> is the implication <m>\neg\mathcal{P}\implies\neg\mathcal{Q}</m>. Neither the converse nor the inverse is equivalent to the original implication, and thus neither of these can be used to give an indirect proof of <m>\mathcal{P}\implies \mathcal{Q}</m>. (Exercise: use a truth table to show that neither the converse nor the inverse implication is logically equivalent to the original implication. )
      </p>
    </statement>
  </warning>

  </subsubsection>
  <subsubsection xml:id="sss_disjunction">
    <title>Disjunction</title>
    <p>
      Again, using <xref ref="d_logical_ops"/>, to directly show a disjunction <m>\mathcal{P}\text{ or }\mathcal{Q}</m> is true, we need only show one the two component propositions is true.
    </p>
    <p>
      Alternatively, we can prove either of the implications <m>\neg\mathcal{P}\implies\mathcal{Q}</m> or <m>\neg Q\implies \mathcal{P}</m>, both of which are logically equivalent to <m>\mathcal{P}\text{ or }\mathcal{Q}</m>. (Exercise: use a truth table to show these three propositions are indeed equivalent!)
    </p>
  </subsubsection>
  <subsubsection xml:id="sss_equivalence">
    <title>Equivalence</title>
    The equivalence <m>\mathcal{P}\iff\mathcal{Q}</m> is logically equivalent to the conjunction
    <me>
      (\mathcal{P}\implies\mathcal{Q})\text{ and } (\mathcal{Q}\implies \mathcal{P})
    </me>.
     Accordingly, the standard way of proving <m>\mathcal{P}\iff \mathcal{Q}</m> is to prove the two implications  <m>\mathcal{P}\implies\mathcal{Q}</m> and <m>\mathcal{Q}\implies\mathcal{P}</m> separately. (Exercise: use a truth table to show these propositions are indeed equivalent!)
  </subsubsection>
  <subsubsection xml:id="sss_logical_chains">
    <title>Chains of implications/equivalences</title>
    <p>
      The relation <q><m>\mathcal{P}</m> implies <m>\mathcal{Q}</m></q> is transitive: <ie />, if <m>\mathcal{P}\implies\mathcal{Q}</m> and <m>\mathcal{Q}\implies\mathcal{R}</m>, then <m>\mathcal{P}\implies\mathcal{R}</m>. Similarly, the relation <q><m>\mathcal{P}</m> is equivalent to <m>\mathcal{Q}</m></q> is transitive. This allows us to prove an implication or equivalence via a <em>chain of implications</em> or <em>chain of equivalences</em>. When writing up a proof using this technique, use a vertically aligned format like the example below, treating one implication or equivalence per line, and adding a brief justification to the right:
      <figure>
        <md>
          <mrow>\mathcal{P} \amp \iff \mathcal{P_1}\amp\text{(justification)}</mrow>
          <mrow> \amp \iff \mathcal{P_2}\amp\text{(justification)} </mrow>
          <mrow> \amp \vdots</mrow>
          <mrow>  \amp \iff \mathcal{P_n}\amp\text{(justification)} </mrow>
          <mrow>  \amp \iff \mathcal{Q}\amp\text{(justification)}</mrow>
        </md>.
        <caption>Proving the equivalence <m>\mathcal{P}\iff \mathcal{Q}</m> via chain of equivalences.</caption>
      </figure>
      It is also possible to build an argument as a hybrid chain of equivalences and implications. In this case the chain is only as strong as its weakest link. For example, a chain of the form
      <md>
        <mrow>\mathcal{P} \amp\iff\mathcal{Q} \amp\text{(justification)} </mrow>
        <mrow> \amp\implies \mathcal{R} \amp\text{(justification)} </mrow>
        <mrow>  \amp\iff \mathcal{S} \amp\text{(justification)}</mrow>
      </md>
      only shows that <m>\mathcal{P}\implies\mathcal{S}</m>. Indeed, we will have <m>\mathcal{P}\iff\mathcal{S}</m> if and only if the intervening implication <m>\mathcal{Q}\implies\mathcal{R}</m> is in fact an equivalence (<ie />, the arrow goes both ways).
    </p>
    <warning>
      <statement>
        <p>
          It is often tempting, for the sake of space, to try and prove an equivalence <m>\mathcal{P}\iff\mathcal{Q}</m> via a chain of equivalences, as opposed to showing <m>\mathcal{P}\implies \mathcal{Q}</m> and <m>\mathcal{Q}\implies\mathcal{P}</m> separately.

          When proceeding in this manner, make doubly sure that each <m>\iff</m> is indeed an equivalence: <ie />, that the implication arrow really goes both ways at each step. Even if each step in your chain truly is an equivalence, you should consider whether this will be obvious to your reader.
        </p>
      </statement>
    </warning>
  <p>
    The example below provides the proof that a function is invertible if and only if it is bijective (<xref ref="th_invertible_bijective"/>). The proof nicely illustrates some of the different techniques used for proving implications and equivalences. Additionally, it is a nice example of how to separate out cases of the argument into clearly distinguished steps.
  </p>
  <example xml:id="ex_invertible_bijective">
    <title>Proof: invertible is equivalent to bijective</title>

    <statement>
      <p>
      Let <m>f\colon A\rightarrow B</m> be a function. Prove: <m>f</m> is invertible if and only if <m>f</m> is bijective.
      </p>
    </statement>
    <solution>
      <p>
       Let <m>\mathcal{P}</m> be the proposition that <m>f</m> is invertible, and let <m>\mathcal{Q}</m> be the proposition that <m>f</m> is bijective. We prove the equivalence <m>\mathcal{P}\iff \mathcal{Q}</m> by proving the two implications <m>\mathcal{P}\implies \mathcal{Q}</m> and <m>\mathcal{Q}\implies\mathcal{P}</m>.
      </p>
      <case>
       <title><m>\mathcal{P}\implies \mathcal{Q}</m></title>
      <p>
      We must show that if <m>f</m> is invertible, then <m>f</m> is bijective. Assume <m>f</m> is invertible. Then <m>f</m> has an inverse <m>f^{-1}</m>. We show separately that <m>f</m> is injective and surjective, hence bijective.
      </p>
      <case>
       <title><m>f</m> is injective</title>
      <p>
        We show <m>f(a)=f(a')\implies a=a'</m> via a chain of implications:
        <md>
          <mrow>f(a)=f(a') \amp \implies f^{-1}(f(a))=f^{-1}(f(a'))</mrow>
          <mrow> \amp\implies a=a' \amp (f^{-1}\circ f=\id_A) </mrow>
        </md>.
      </p>
      </case>
      <case>
       <title><m>f</m> is surjective</title>
      <p>
        Let <m>b</m> be an element of <m>B</m>. We must show that there is an <m>a\in A</m> such that <m>f(a)=b</m>. Letting <m>a=f^{-1}(b)</m>, we have
        <md>
          <mrow>f(a) \amp = f(f^{-1}(b))</mrow>
          <mrow> \amp = b \amp (f\circ f^{-1}=\id_B)</mrow>
        </md>.
      </p>
      </case>
      </case>
      <case>
       <title><m>\mathcal{Q}\implies\mathcal{P}</m></title>
      <p>
      We must show that if <m>f</m> is bijective, then <m>f</m> is invertible. Assume <m>f</m> is bijective. First we define a function <m>g\colon B\rightarrow A</m> as follows: for all <m>b\in B</m>, let <m>g(b)</m> be the unique element <m>a\in A</m> such that <m>f(a)=b</m>. Note that our definition of <m>g</m> uses both that <m>f</m> is surjective (there is <em>some</em> element <m>a</m> such that <m>f(a)=b</m>)) and injective (there is <em>exactly one</em> element <m>a</m> such that <m>f(a)=b</m>).
      </p>
      <p>
        We now prove that <m>g</m> is the inverse of <m>f</m>, showing <m>g\circ f=\id_A</m> and <m>f\circ g=\id_B</m> separately.
      </p>
      <case>
       <title><m>g\circ f=\id_A</m></title>
      <p>
      Take any <m>a\in A</m> and let <m>b=f(a)</m>. By definition of <m>g</m>, we have <m>g(b)=a</m> and hence <m>g(f(a))=g(b)=a</m>. This proves <m>g\circ f=\id_A</m>.
      </p>
      </case>
      <case>
       <title><m>f\circ g=\id_B</m></title>
      <p>
      Take any <m>b\in B</m>. By definition of <m>g</m>, <m>g(b)</m> is the unique <m>a\in A</m> such that <m>f(a)=b</m>. Thus <m>f(g(b))=f(a)=b</m>. This proves <m>f\circ g=\id_B</m>.
      </p>
      </case>
      </case>
    </solution>
  </example>
  </subsubsection>
  <subsubsection xml:id="sss_proof_by_contradiction">
    <title>Proof by contradiction</title>
    The technique of <em>proof by contradiction</em> (or <em>reductio ad absurdum</em>) proves a proposition <m>\mathcal{P}</m> by (a) assuming the negation <m>\neg\mathcal{P}</m> is true, and then (b) using this assumption to derive a proposition <m>\mathcal{Q}</m> known to be false. The choice of falsehood <m>\mathcal{Q}</m> is completely up to the person providing the proof. However, in order for the proof to be convincing, it should be clear, either logically or because of theory assumed to be known, that <m>\mathcal{Q}</m> is indeed false.
    <example xml:id="ex_proof_by_contradiction">
      <title>Proof by contradiction</title>
      <statement>
        <p>
        Prove by contradiction that <m>0</m> has no multiplicative inverse in the reals: <ie />, there is no <m>r\in\R</m> such that <m>r\cdot 0=1</m>.
        </p>
      </statement>
      <solution>
        <p>
          We prove the claim by contradiction. Assume there is an <m>r\in \R</m> such that <m>r\cdot 0=1</m>. Since <m>r\cdot 0=0</m> for any <m>r\in \R</m> (a property of multiplication by 0), we have <m>1=r\cdot 0=0</m>: a contradiction since <m>1\ne 0</m>. We conclude that there is no <m>r\in \R</m> such that <m>r\cdot 0=1</m>.
        </p>
      </solution>
    </example>
        <remark xml:id="rm_proof_by_contradiction">
      <statement>
        <p>
          Proof by contradiction resembles, but is not quite the same  thing as proving an implication via its contrapositive. Letting <m>F</m> denote an arbitrary falsehood (the <m>\mathcal{Q}</m> described above) what we do in a proof by contradiction is show that the implication <m>\neg \mathcal{P}\implies F</m> is true. Since <m>F</m> is false, and the implication is true, <m>\neg \mathcal{P}</m> must be false: equivalently, <m>\mathcal{P}</m> must be true.
        </p>
      </statement>
    </remark>
    </subsubsection>
</subsection>
<subsection xml:id="ss_set_properties">
  <title>Basic set properties</title>
<subsubsection xml:id="sss_set_inclusion">
  <title>Set inclusion</title>
  <p>
    Let <m>A</m> and <m>B</m> be sets. By <xref ref="d_set_inclusion"/>, to prove <m>A\subseteq B</m> we must show that for all elements <m>x</m> we have
  <me>
    x\in A\implies x\in B
  </me>.
  This requires proving the implication above for a general element <m>x</m>, and we may use any of  the techniques described in <xref ref="sss_implication" text="title"/> and <xref ref="sss_logical_chains" text="title"/> to do so. 
</p>
</subsubsection>
<subsubsection xml:id="sss_set_equality">
  <title>Set equality</title>
  <p>
    Let <m>A</m> and <m>B</m> be sets. To prove <m>A=B</m> directly using <xref ref="d_set_equality"/> we must show that for all elements <m>x</m> we have
    <me>
      x\in A \iff x\in B
    </me>.
     To prove this universal equivalence, we must give an argument for the equivalence that holds for a general element <m>x</m>.
  </p>
  <p>
    Alternatively, you can prove <m>A=B</m> by proving the two set inclusions <m>A\subseteq B</m> and <m>B\subseteq A</m> separately. This is equivalent to proving the two implications <m>x\in A\implies x\in B</m> and <m>x\in B\implies x\in A</m> separately.
  </p>
</subsubsection>
</subsection>


</section>
